reorganised stepping; start of writing c0 tactics

C0deine/Experimental/Prover.lean
@@ -4,6 +4,9 @@
  -/
 import C0deine.Top
 import C0deine.Type.SyntaxTree.Dynamics
+import C0deine.Type.SyntaxTree.Dynamics.Notation
+import C0deine.Type.SyntaxTree.Dynamics.Transitivity
+import C0deine.Ast.Ast
 
 namespace C0deine.Prover
 
@@ -42,3 +45,83 @@ int main() {
 
 #eval (prog₁ >>= (fun (tst, _ctx) => pure (toString tst))).run ()
 
+def test_ast := Ast.Expr.binop (.int .plus) (.num 5) (.num 5)
+
+macro "c0_step_expr_setup" : tactic =>
+  `(tactic| ( apply Tst.Dynamics.Steps.trans
+              apply Exists.intro 1
+              apply Tst.Dynamics.Step.expr
+            )
+   )
+
+macro "c0_step_self" : tactic => `(tactic| exact ⟨0, by rfl⟩)
+
+macro "c0_step_one_setup" : tactic =>
+  `(tactic| ( apply Tst.Dynamics.Steps.trans
+              apply Exists.intro 1
+            )
+   )
+
+elab "c0_step" : tactic =>
+  Lean.Elab.Tactic.withMainContext do
+    let goal ← Lean.Elab.Tactic.getMainGoal
+    let goal_type ← goal.getType''
+
+    -- check if we need to split a sequence of steps into one step
+    if goal_type.isAppOf `C0deine.Tst.Dynamics.Steps then
+      Lean.Elab.Tactic.evalTactic (← `(tactic| try c0_step_self))
+
+      if (← Lean.Elab.Tactic.getGoals).isEmpty then return
+      -- could not step to self, there must be one more step
+      Lean.Elab.Tactic.evalTactic (← `(tactic| c0_step_one_setup))
+
+    -- try stepping the code
+    let get_dyn_res : Lean.Expr → _ :=
+      fun goal_type => do (← goal_type.getArg? 1).getArg? 4
+
+    let goal ← Lean.Elab.Tactic.getMainGoal
+    let goal_type ← goal.getType'
+    let dyn_res ← get_dyn_res goal_type
+    
+    match dyn_res.getAppFn with
+    | .const `C0deine.Tst.Dynamics.DynResult.val _
+    | .const `C0deine.Tst.Dynamics.DynResult.eval _ =>
+      Lean.Elab.Tactic.evalTactic (← `(tactic| apply Tst.Dynamics.Step.expr))
+      let goal ← Lean.Elab.Tactic.getMainGoal
+      let goal_type ← goal.getType'
+      let dyn_res ← get_dyn_res goal_type
+      let expr ← dyn_res.getArg? 4
+      
+      match expr.getAppFn with
+      | .const expr_name _ =>
+        match expr_name.componentsRev with
+        | `binop_int :: _
+        | `binop_int₁ :: _ =>
+          Lean.Elab.Tactic.evalTactic (← `(tactic| apply Tst.Dynamics.Step.Expr.binop))
+          Lean.Elab.Tactic.evalTactic (← `(tactic| constructor))
+        | `binop_int₂ :: _ =>
+          Lean.Elab.Tactic.evalTactic (← `(tactic| apply Tst.Dynamics.Step.Expr.binop))
+          Lean.Elab.Tactic.evalTactic (← `(tactic| constructor))
+          Lean.Elab.Tactic.evalTactic (← `(tactic| constructor))
+        | test =>
+          -- dbg_trace f!"Expr name: {expr_name}"
+          -- dbg_trace f!"Expr name last: {test}"
+          Lean.Elab.Tactic.evalTactic (← `(tactic| constructor))
+      | _ =>
+        Lean.Meta.throwTacticEx `c0_step goal "Could not find C0 dynamic state"
+    | dyn_mode =>
+      dbg_trace f!"TODO: {dyn_mode} | type: {goal_type}"
+    -- dbg_trace f!""
+
+open Typ.Notation in
+def tst : Tst.Expr {} {} (int) :=
+  Tst.Expr.binop_int (by rfl) (by rfl) (by rfl)
+    .plus (.num (by rfl) 5) (.num (by rfl) 5)
+
+open Tst.Dynamics Notation in
+example /-  5 + 5 ==>* 10   -/
+       : (H; S; η |= (.eval tst .nil)                       [prog|p])
+    ==>* (H; S; η |= (.val (Δ:={}) (Γ:={}) (.num 10) .nil)  [prog|p])
+    := by
+  rw [tst]
+  repeat c0_step
