C0deine/Type/SyntaxTree/Dynamics/Notation.lean
@@ -6,6 +6,9 @@ import C0deine.Type.SyntaxTree.Dynamics.Step
 
 namespace C0deine.Tst.Dynamics.Notation
 
-scoped notation:50 H:51 " ; " S:51 " ; " η:51 " |= " r:51 => State.mk H S η r
+scoped notation:50 H:51 " ; " S:51 " ; " η:51 " |= " r:51 " [prog| " p:51 " ] " =>
+  State.mk (p:=p) H S η r
 scoped notation:50 s₁:51 " ==> " s₂:51 => Step s₁ s₂
 scoped notation:50 s₁:51 " ==>* " s₂:51 => Steps s₁ s₂
+
+-- scoped notation:50 e:51 "▷" K:51 => DynResult.eval e K
